proof/examples/zk/abstract/Abstract_exp_proof_8.ec
@@ -9,7 +9,7 @@ require Abstract_exp_proof_7.
 clone include Abstract_exp_proof_7.
 
 import IterOp.
-import Zp.
+
 
 module M8 = {
   proc expm_spec (x:R, n:R) : R = {
@@ -17,48 +17,6 @@ module M8 = {
   }  
 }.
 
-
-lemma kk :  forall (n : int), 0 <= n => forall (a : zp) (b : R), valR b < P =>
-  ImplFp b a =>
-  ImplFp (b ^ n) (inzp (asint a ^ n)).
-apply intind. progress. 
-rewrite exp_prop1.
-have -> : (asint a ^ 0) = 1. smt.
-rewrite /asint.
-have -> : (Sub.val (inzp 1))%Sub = 1. smt.
-smt(valR_one).
-progress.
-have ->: (b ^ (i + 1)) = b *** (b ^ i).
-rewrite exp_prop3. auto. auto.  auto.
-rewrite exp_prop2.
-rewrite exp_prop7. auto.
-have ->: inzp (asint a ^ (i + 1)) =  inzp (asint a * (asint a ^ i)).
-smt.
-have ->:  inzp (asint a * (asint a ^ i)) = (inzp (asint a)) * (inzp (asint a ^ i)).
-smt.
-rewrite - H2.
-have ->: asint (inzp (valR b) * inzp (valR b ^ i))
-  = (asint (inzp (valR b)) * (asint  (inzp (valR b ^ i)))) %% P.
-smt.
-have ih :  ImplFp (b ^ i)  (inzp (valR b ^ i)).
-rewrite H2. apply H0. auto. auto.
-rewrite - ih.
-have ->: asint (inzp (valR b)) = valR b. smt.
-have ->: valR (b *** (b ^ i)) =  (valR b) * (valR (b ^ i)) %%P.
-rewrite  to_uintP /=. done.
-auto.
-qed.
-
-
-lemma exp_real_speacc :
- equiv[ Spec.expm ~ M8.expm_spec  : 
-    ImplFp arg{2}.`1 arg{1}.`1 /\ valR arg{2}.`2 = arg{1}.`2 /\ valR x{2} < P ==> ImplFp res{2} res{1}].
-proc. 
-wp.  skip.  progress.
-apply kk.
-smt. auto.
-auto.
-qed.
 
 
 lemma exp_real_speac2 :
@@ -72,7 +30,6 @@ qed.
 section.
 declare module M <: BasicOps.
 
-
 declare axiom exp_swap :
  equiv[ M.swapr ~ Spec.swapr    : arg{2}.`1 = arg{1}.`1 /\ arg{2}.`2 = arg{1}.`2 /\   arg{1}.`3 = as_w64 arg{2}.`3
     ==> ={res}].
@@ -82,26 +39,7 @@ declare axiom exp_ithbit :
     /\ 0 <= ctr{2} < Rsize ==> ={res} /\ (res{2} = W64.one \/ res{2} = W64.zero) ].
 
 
-declare axiom exp_mulm : 
-  equiv [ M.mulm ~ Spec.mulm: valR arg{1}.`2 = asint arg{2}.`1 /\ valR arg{1}.`3 = asint arg{2}.`2 /\ ImplR p{1} P  ==> valR res{1} = asint res{2} ].
-
 declare axiom stateless_M (x y : glob M) : x = y.
-
-lemma exp_mulm2 : 
-  equiv [ M.mulm ~ Spec.mul: arg{1}.`2 = arg{2}.`1 /\ arg{1}.`3 = arg{2}.`2 /\ ImplR p{1} P /\ valR a{1} < P /\ valR b{1} < P  ==> ={res} ].
-transitivity Spec.mulm
-     (valR arg{1}.`2 = asint arg{2}.`1 /\ valR arg{1}.`3 = asint arg{2}.`2 /\ ImplR p{1} P   ==> valR res{1} = asint res{2})
-     (valR arg{2}.`1 = asint arg{1}.`1 /\ valR arg{2}.`2 = asint arg{1}.`2   ==> valR res{2} = asint res{1}).
-progress. 
-exists (inzp (valR a{1}), inzp (valR b{1}) ). progress.
-smt. smt. smt. smt.
-progress. smt.
-conseq exp_mulm. 
-proc. wp. skip. progress.
-have  ->: valR (a{2} *** b{2}) = valR a{2} * valR b{2} %% P. smt.
-have ->: asint (a{1} * b{1}) = asint (a{1})  * asint  b{1} %% P. smt. 
-smt().
-qed.
 
 
 lemma exp_real_speac :
@@ -112,7 +50,7 @@ lemma exp_real_speac :
    /\ valR x{1} < P
      ==> ={res}].
 transitivity M2.expm
-   (={arg} /\  0 < size arg{1}.`2 /\   valR x{1} < P ==> ={res}) 
+   (={arg} /\  0 < size arg{1}.`2  /\   valR x{1} < P  ==> ={res}) 
   (valR arg{2}.`1 = P 
    /\  arg{1}.`1 = arg{2}.`2
    /\ bs2int arg{1}.`2 = valR arg{2}.`3
@@ -165,38 +103,106 @@ smt (stateless_M).
 qed.
 
 
-lemma exp_pre_fin :
- equiv[ Spec.expm ~ M7(M).expm  : 
-       valR arg{2}.`1  = P 
-   /\  ImplFp  arg{2}.`2 arg{1}.`1
-   /\  arg{1}.`2 =  valR arg{2}.`3
-   /\  valR x{2} < P
-     ==> ImplFp res{2} res{1} ].
-transitivity M8.expm_spec
-  (ImplFp arg{2}.`1 arg{1}.`1 /\ valR arg{2}.`2 = arg{1}.`2 /\ valR x{2} < P ==> ImplFp res{2} res{1})
-  (valR arg{2}.`1 = P 
-   /\  arg{1}.`1 = arg{2}.`2
-   /\  arg{1}.`2 =  arg{2}.`3
-   /\ valR x{1} < P
-     ==> ={res}).
-progress. exists (x{2},n{2}). progress. smt(). auto.
-conseq exp_real_speacc.   
-transitivity M1.expm_spec  
-  (arg{1}.`1 = arg{2}.`1 /\ valR arg{1}.`2 = bs2int arg{2}.`2 /\ valR x{2} < P ==> ={res})
-  (valR arg{2}.`1 = P 
-   /\  arg{1}.`1 = arg{2}.`2
-   /\ bs2int arg{1}.`2 = valR arg{2}.`3
-   /\ size arg{1}.`2 = Rsize
-   /\ valR x{1} < P
-     ==> ={res}).
-progress. 
-exists (x{1},  Rbits n{2}).
-progress.
-smt().
-smt(iii).
-smt().
-conseq exp_real_speac2. 
-progress. conseq exp_real_speac.
-qed.
-
 end section.
+
+
+
+
+(* declare axiom exp_mulm :  *)
+(*   equiv [ M.mulm ~ Spec.mulm: valR arg{1}.`2 = asint arg{2}.`1 /\ valR arg{1}.`3 = asint arg{2}.`2 /\ ImplR p{1} P  ==> valR res{1} = asint res{2} ]. *)
+
+(* lemma exp_mulm2 :  *)
+(*   equiv [ M.mulm ~ Spec.mul: arg{1}.`2 = arg{2}.`1 /\ arg{1}.`3 = arg{2}.`2 /\ ImplR p{1} P /\ valR a{1} < P /\ valR b{1} < P  ==> ={res} ]. *)
+(* transitivity Spec.mulm *)
+(*      (valR arg{1}.`2 = asint arg{2}.`1 /\ valR arg{1}.`3 = asint arg{2}.`2 /\ ImplR p{1} P   ==> valR res{1} = asint res{2}) *)
+(*      (valR arg{2}.`1 = asint arg{1}.`1 /\ valR arg{2}.`2 = asint arg{1}.`2   ==> valR res{2} = asint res{1}). *)
+(* progress.  *)
+(* exists (inzp (valR a{1}), inzp (valR b{1}) ). progress. *)
+(* smt. smt. smt. smt. *)
+(* progress. smt. *)
+(* conseq exp_mulm.  *)
+(* proc. wp. skip. progress. *)
+(* have  ->: valR (a{2} *** b{2}) = valR a{2} * valR b{2} %% P. smt. *)
+(* have ->: asint (a{1} * b{1}) = asint (a{1})  * asint  b{1} %% P. smt.  *)
+(* smt(). *)
+(* qed. *)
+
+
+(* import Zp. *)
+
+(* lemma kk :  forall (n : int), 0 <= n => forall (a : zp) (b : R), valR b < P => *)
+(*   ImplFp b a => *)
+(*   ImplFp (b ^ n) (inzp (asint a ^ n)). *)
+(* apply intind. progress.  *)
+(* rewrite exp_prop1. *)
+(* have -> : (asint a ^ 0) = 1. smt. *)
+(* rewrite /asint. *)
+(* have -> : (Sub.val (inzp 1))%Sub = 1. smt. *)
+(* smt(valR_one). *)
+(* progress. *)
+(* have ->: (b ^ (i + 1)) = b *** (b ^ i). *)
+(* rewrite exp_prop3. auto. auto.  auto. *)
+(* rewrite exp_prop2. *)
+(* rewrite exp_prop7. auto. *)
+(* have ->: inzp (asint a ^ (i + 1)) =  inzp (asint a * (asint a ^ i)). *)
+(* smt. *)
+(* have ->:  inzp (asint a * (asint a ^ i)) = (inzp (asint a)) * (inzp (asint a ^ i)). *)
+(* smt. *)
+(* rewrite - H2. *)
+(* have ->: asint (inzp (valR b) * inzp (valR b ^ i)) *)
+(*   = (asint (inzp (valR b)) * (asint  (inzp (valR b ^ i)))) %% P. *)
+(* smt. *)
+(* have ih :  ImplFp (b ^ i)  (inzp (valR b ^ i)). *)
+(* rewrite H2. apply H0. auto. auto. *)
+(* rewrite - ih. *)
+(* have ->: asint (inzp (valR b)) = valR b. smt. *)
+(* have ->: valR (b *** (b ^ i)) =  (valR b) * (valR (b ^ i)) %%P. *)
+(* rewrite  to_uintP /=. done. *)
+(* auto. *)
+(* qed. *)
+
+
+(* lemma exp_real_speacc : *)
+(*  equiv[ Spec.expm ~ M8.expm_spec  :  *)
+(*     ImplFp arg{2}.`1 arg{1}.`1 /\ valR arg{2}.`2 = arg{1}.`2 /\ valR x{2} < P ==> ImplFp res{2} res{1}]. *)
+(* proc.  *)
+(* wp.  skip.  progress. *)
+(* apply kk. *)
+(* smt. auto. *)
+(* auto. *)
+(* qed. *)
+
+
+
+(* lemma exp_pre_fin : *)
+(*  equiv[ Spec.expm ~ M7(M).expm  :  *)
+(*        valR arg{2}.`1  = P  *)
+(*    /\  ImplFp  arg{2}.`2 arg{1}.`1 *)
+(*    /\  arg{1}.`2 =  valR arg{2}.`3 *)
+(*      ==> ImplFp res{2} res{1} ]. *)
+(* transitivity M8.expm_spec *)
+(*   (ImplFp arg{2}.`1 arg{1}.`1 /\ valR arg{2}.`2 = arg{1}.`2 /\ valR x{2} < P ==> ImplFp res{2} res{1}) *)
+(*   (valR arg{2}.`1 = P  *)
+(*    /\  arg{1}.`1 = arg{2}.`2 *)
+(*    /\  arg{1}.`2 =  arg{2}.`3 *)
+(*    /\ valR x{1} < P *)
+(*      ==> ={res}). *)
+(* progress. exists (x{2},n{2}). progress. smt(). smt.  smt. auto. *)
+(* conseq exp_real_speacc.    *)
+(* transitivity M1.expm_spec   *)
+(*   (arg{1}.`1 = arg{2}.`1 /\ valR arg{1}.`2 = bs2int arg{2}.`2 /\ valR x{2} < P ==> ={res}) *)
+(*   (valR arg{2}.`1 = P  *)
+(*    /\  arg{1}.`1 = arg{2}.`2 *)
+(*    /\ bs2int arg{1}.`2 = valR arg{2}.`3 *)
+(*    /\ size arg{1}.`2 = Rsize *)
+(*    /\ valR x{1} < P *)
+(*      ==> ={res}). *)
+(* progress.  *)
+(* exists (x{1},  Rbits n{2}). *)
+(* progress. *)
+(* smt(). *)
+(* smt(iii). *)
+(* smt(). *)
+(* conseq exp_real_speac2.  *)
+(* progress. conseq exp_real_speac. *)
+(* qed. *)
